P1_UInt32.fst
@@ -27,7 +27,7 @@ let unpack_tree = NTreeC3.unpack_tree #U32.t
 //inline_for_extraction
 //let intro_linked_tree_leaf = NTreeC3.intro_linked_tree_leaf #U32.t
 
-let elim_linked_tree_leaf = NTreeC3.elim_linked_tree_leaf #U32.t
+//let elim_linked_tree_leaf = NTreeC3.elim_linked_tree_leaf #U32.t
 let create_leaf = NTreeC3.create_leaf #U32.t
 
 //noextract
